   $\begin{aligned}
      f(x)&=(x+a)(x+b)\\
          &=x^2+(a+b)x+ab
   \end{aligned}$
   $\begin{alignedat}
          f(x)&=(x+a)(x+b)\\
              &=x^2+(a+b)x+ab
   \end{alignedat}$
   $u(x)=
   \begin{cases}
      \exp{x} & \text{if } x \geq 0 \\
   1       & \text{if } x < 0   
   \end{cases}$
```{matlab}
x = 1:100;
s=0;
y =circshift(X)
```
```{python}
print(X)
a = list
```
$\frac{a}{b}$

$\begin{aligned}
   \sum_{n=0}^{N-1}n^2
\end{aligned}$



$\begin{bmatrix}
    x_{11}       & x_{12} & x_{13} & \dots & x_{1n} \\
    x_{21}       & x_{22} & x_{23} & \dots & x_{2n} \\
    \vdots & \vdots & \vdots & \ddots & \vdots  \\
    x_{d1}       & x_{d2} & x_{d3} & \dots & x_{dn}
\end{bmatrix}$
=
$\begin{bmatrix}
    x_{11} & x_{12} & x_{13} & \dots  & x_{1n} \\
    x_{21} & x_{22} & x_{23} & \dots  & x_{2n} \\
    \vdots & \vdots & \vdots & \ddots & \vdots \\
    x_{d1} & x_{d2} & x_{d3} & \dots  & x_{dn}
\end{bmatrix}$

$\begin{Bmatrix}
   x_{11}&x_{12}&x_{13}\\
   x_{21}&x_{22}&x_{23}
\end{Bmatrix}$  

$\begin{cases}
   a>0&a-b\\a<0&a+b
\end{cases}$  

$\begin{aligned}
   (X^TX)^{-1}&=
   \end{aligned}
   \begin{aligned}
   \frac{1}{n\sum_{i=1}^n X_i^2 - \left(\sum_{i=1}^n X_i\right)^2}
\end{aligned} 
\begin{pmatrix}
\sum_{i=1}^n X_i^2 & -\sum_{i=1}^n Xi\\
  \sum _{i=1}^n X_i & n
\end{pmatrix}
\begin{aligned}
&=\frac{1}{n \sum _{i=1}^n X_i^2 - ( \sum X_i)^2} 
\left[n \sum_{i=1}^n X_i^2 - \left( \sum _{i=1} ^n X_i\right)^2\right]
\\
 &=1\end{aligned}$
 $\mathscr{R}$




